
\begin{align*}
e^{\Phi} & =
\frac{c \sin^2\phi \, X_1+\cos^2\phi \,X_2}{\sqrt{c X_1 X_2}}\\
%
C_{(0)} & = 
-\frac{\sin(2 \phi ) (c X_1-X_2)}{2  (c \sin^2\phi \, X_1+\cos^2\phi \,X_2)}\\
%
C_{(2)} & = 
- a_2 \sin\phi \,
\sigma_2\wedge \sigma_3
+ a_3 \cos\phi \,
\sigma_1\wedge d\phi
+ a_1 \sin\phi \,
\sigma_1\wedge d\theta\\
% 
B_{(2)} & =
a_2 \cos\phi \,
\sigma_2\wedge \sigma_3
+ a_3 \sin\phi \,
\sigma_1\wedge d\phi
- a_1 \cos\phi \,
\sigma_1\wedge d\theta\\
% 
C_{(4)} & =
4 \, \omega \,
dx_0\wedge dx_1\wedge dx_2\wedge dx_3 
+ \sin\phi \cos\phi \, a_1 a_2 \,
d\theta\wedge \sigma_1\wedge \sigma_2\wedge \sigma_3\\
&
-\left(\cos ^2\phi \, a_2 a_3 +\frac{c \cos^4\theta}{X_2}\right) 
\sigma_1\wedge \sigma_2\wedge \sigma_3 \wedge d\phi \\
%
C_{(6)} &= - C_{(4)} \wedge B_{(2)}\\
&+\frac{(c A-2) A \sin\theta \cos^2\theta \cos\phi}{2 \left(c^2-1\right)^{5/2}} 
\sigma_1\wedge dc\wedge dx_0\wedge dx_1\wedge dx_2\wedge dx_3\\
&
+\frac{A^2 \cos^3\theta \cos\phi}{2 (c^2-1)^{3/2}}
\sigma_1\wedge dx_0 \wedge dx_1\wedge dx_2\wedge dx_3\wedge d\theta\\
&
-\frac{A^2 \sin\theta \cos^2\theta \sin\phi}{2 (c^2-1)^{3/2}}
\sigma_1\wedge dx_0 \wedge dx_1\wedge dx_2\wedge dx_3\wedge d\phi\\
%
C_{(8)} &= - C_{(6)} \wedge B_{(2)}\\
&+ \left\{ \frac{A \sin^2\theta \cos^4\theta \cos(2\phi) \left[ ((c^2+3) A-4 c) \cos^2\theta-2 A \right]}{4 (c^2-1)^2 X_2^2} \right.\\
&+ \left.\frac{A ((c^2-1) A + 4 c) \cos^4\theta}{8 c^2 (c^2-1)^2} \right\}
\sigma_1 \wedge \sigma_2\wedge \sigma_3\wedge dc\wedge dx_0\wedge dx_1\wedge dx_2\wedge dx_3\\
& -\frac{A^2 \sin^3(2 \theta ) \cos(2 \phi ) \left(2 c A + A^2 \sin^2\theta +c^2 \cos^2\theta\right)}{16 c (c^2-1) X_2^2}\\
&\sigma_1\wedge \sigma_2\wedge \sigma_3\wedge dx_0\wedge dx_1\wedge dx_2\wedge dx_3\wedge d\theta
\end{align*}
