
The Killing spinor solution $\epsilon$, originally derived in \cite{Pilch:2003jg} and we follow the appendix of \cite{Chen-Lin:2015xlh}, has the following expression:
\begin{align}
\epsilon &= \Omega^{1/2} \exp{\left(\frac{\phi}{2}\, i \right)} \exp{\left(\frac{\alpha}{2}\Gamma_{56} \right)} \exp{\left(\frac{\beta}{2}\Gamma_{7 10} \mathcal{K} \right)} \eta
\end{align}
where we defined
\begin{equation}
\eta \equiv \Pi_{+} \mathcal{P}_+ \epsilon_0
\end{equation}
and the constant spinor $\epsilon_0$ satisfies
\begin{equation}
 \Pi_+ \mathcal{P}_+ \epsilon_0 = \epsilon_0.
\end{equation}

The projectors are
\begin{align}
\Pi_\pm = 
\frac{1}{2}\left(1 \pm i\Gamma_{1234}\right), 
\quad
\mathcal{P}_{\pm} =
\dfrac{1}{2} \left(1\pm i\Gamma_{6 10}\right),
\end{align}
and they commute with each other: $[\Pi_\pm, \mathcal{P}_{\pm}]=0$. 
% They provide some useful identities:
% \begin{align}
%  & \mathcal{P}_- \eta = 0 \quad \Rightarrow \quad \Gamma_{6,10} \eta = -i \eta \\
%  & \Pi_- \eta = 0 \quad \Rightarrow \quad \Gamma_{1,2,3,4} \eta = -i \eta
% \end{align}


The exponentials can be written in terms of cosines and sines:
\begin{align}
&\exp{\left(\frac{\alpha}{2}\Gamma_{56} \right)} = \cos\frac{\alpha}{2} + \sin\frac{\alpha}{2}\Gamma_{5 6},\\
&\exp{\left(\frac{\beta}{2}\Gamma_{7 10} \mathcal{K} \right)} = \cos\frac{\beta}{2} + \sin\frac{\beta}{2}\Gamma_{7 10}\mathcal{K},
\end{align}
where $\mathcal{K}$ is complex conjugation, and the angles are defined as
\begin{align}
\cos\beta = \sqrt{\frac{X_1}{c X_2}}, \quad 
&\quad
\sin\beta = -\sqrt{\frac{c^2 - 1}{c X_2}}\cos\theta\\
%
\cos\alpha = \frac{\cos\theta}{\sqrt{X_1}}, 
&\quad
\sin\alpha = \sqrt{\frac{c A}{X_1}}\sin\theta,
\end{align}
where $\Omega, X_{1,2}, A$ are functions of $c$ and $\theta$ defined in section \ref{sec:metric}.


The gamma matrices are in real representations. It is convenient to write the $e^{i \frac{\phi}{2}}$ factor in real representation too. 
That is achieved by using $\mathcal{P}_- \eta = 0 $, which leads to
\begin{align}
 \exp{\left(\frac{\phi}{2}\, i \right)} \eta 
    = \exp{\left(-\frac{\phi}{2}\Gamma_{6 10} \right)} \eta. 
\end{align}

After some straightforward manipulations, the Killing spinor can be rewritten as:
\begin{equation}\label{eq:KillingSpinor}
\epsilon =  \Omega^{1/2} \exp{\left(\frac{\alpha}{2}\Gamma_{56} \right)} \exp{\left(-\frac{\phi}{2}\, \Gamma_{6 10} \right)} \exp{\left(\frac{\beta}{2}\Gamma_{7 10} \mathcal{K} \right)} \Pi_{+} \mathcal{P}_+ \epsilon_0.
\end{equation}

